\section{Crowd dynamics}
\subsection{Parameters}
Vector norm and inner product
\begin{align}
\left\langle \mathbf{x}, \mathbf{x} \right\rangle &= \mathbf{x} \cdot \mathbf{x} = \left\| \mathbf{x}\right\|^{2}
\end{align}
Unit vector
\begin{align}
\hat{\mathbf{e}} = \frac{\mathbf{e}}{\left\|\mathbf{e}\right\|}
\end{align}

\begin{align}
\mathbf{x}_{i} &= \text{Centre of mass of agent } i \\
\mathbf{v}_{i} &= \text{Velocity of agent } i \\
r_{i} &= \text{Radius of agent } i \\
m_{i} &= \text{Mass of agent } i
\end{align}

\begin{align}
\mathbf{x}_{ij} &= \mathbf{x}_{i} - \mathbf{x}_{j} \\
\mathbf{v}_{ij} &= \mathbf{v}_{i} - \mathbf{v}_{j} \\
r_{ij} &= r_{i} + r_{j} \\
d_{ij} &= \left\|\mathbf{x}_{ij}\right\|
\end{align}

\begin{align}
a &= \mathbf{v}_{ij} \cdot \mathbf{v}_{ij} \\
b &= -\mathbf{x}_{ij} \cdot \mathbf{v}_{ij} \\
c &= d_{ij}^{2} - r_{ij}^{2} \\
d &= \sqrt{b^{2} - a c} \\
\tau &= \frac{b - \sqrt{d}}{a} > 0
\end{align}

\begin{align}
h_{ij} &= r_{ij} - d_{ij} \\
h_{iw} &= r_{i} - d_{iw}
\end{align}

\begin{align}
\mathbf{n}_{ij} &= \frac{\mathbf{x}_{ij}}{d_{ij}} \\
\mathbf{t}_{ij} &= R(-45^{\circ}) \cdot \mathbf{n}_{ij} \\
%\Delta \mathbf{v}_{ji}^{t} &= \mathbf{v}_{ji} \cdot \mathbf{t}_{ij}
\end{align}

\subsection{Social force model}
Total force on the agent $ i $
\begin{align}
\mathbf{f}_{i}(t) = \mathbf{f}_{i}^{adj} + \sum_{j\neq i}^{} \left(\mathbf{f}_{ij}^{soc} + \mathbf{f}_{ij}^{c}\right) + \sum_{w}^{} \left(\mathbf{f}_{iw}^{soc} + \mathbf{f}_{iw}^{c}\right) + \boldsymbol{\xi}_{i}
\end{align}

\begin{enumerate}[label=\roman{enumi})]
\item 
Force adjusting agent's movement towards desired in some characteristic time $ \tau_{i}^{adj} $
\begin{align}
\mathbf{f}_{i}^{adj} &= \frac{m_{i}}{\tau_{i}^{adj}} (\mathbf{v}_{i}^{0} - \mathbf{v}_{i}) 
\end{align}
Target velocity can be broken down
\begin{align}
\mathbf{v}_{i}^{0} &= v_{i}^{0} \cdot \hat{\mathbf{e}}_{i}^{0}
\end{align}
Target direction
\begin{align}
\mathbf{e}_{i}^{0}(t) &= (1 - p_{i})\mathbf{e}_{i} + p_{i} \left\langle \mathbf{e}_{j}^{0}(t) \right\rangle_{i} \\
\hat{\mathbf{e}}_{i}^{0}(t) &= \frac{\mathbf{e}_{i}^{0}(t)}{\left\| \mathbf{e}_{i}^{0}(t) \right\|}
\end{align}

\item 
Psychological tendency to keep a certain distance to other agents
\begin{align}
\mathbf{f}_{ij}^{soc} &=
\begin{cases}
\mathbf{f}_{ij}^{pow} &  d_{ij} \leq sight \\
0 & \text{otherwise}
\end{cases}
\end{align}
and walls
\begin{align}
\mathbf{f}_{iw}^{soc} &= A_{i} \exp\left(\frac{h_{iw}}{B_{i}}\right) \mathbf{n}_{iw}
\end{align} 


\item 
Physical contact forces with other agents 
\begin{align}
\mathbf{f}_{ij}^{c} &= 
\begin{cases}
h_{ij} \left(\mu \cdot \mathbf{n}_{ij} - \kappa \cdot \left(\mathbf{v}_{ji} \cdot \mathbf{t}_{ij}\right) \mathbf{t}_{ij}\right) & h_{ij} > 0 \\
0 & \text{otherwise}
\end{cases}
\end{align}
and walls
\begin{align}
\mathbf{f}_{iw}^{c} &= 
\begin{cases}
h_{iw} \left(\mu \cdot \mathbf{n}_{iw} - \kappa \cdot (\mathbf{v}_{i} \cdot \mathbf{t}_{iw}) \mathbf{t}_{iw}\right) & h_{iw} > 0 \\
0 & \text{otherwise}
\end{cases}
\end{align}


\item 
Uniformly distributed random fluctuation force
\begin{align}
\boldsymbol{\xi}_{i} &= \boldsymbol{\mathcal{U}}(-1, 1).
\end{align}


\end{enumerate}


\subsection{Universal power law governing pedestrian interactions}
Interaction force between agents
\begin{align}
\mathbf{f}_{ij}^{pow} &= -\nabla_{\mathbf{x}_{ij}} E(\tau) 
= -\nabla_{\mathbf{x}_{ij}} \left(\frac{k}{\tau^{2}} \exp \left( -\frac{\tau}{\tau_{0}} \right) \right) \\
%\\
%&= - \left[\frac{k}{\left\|\mathbf{v}_{ij}\right\|^{2} \tau^{2}} \exp \left( -\frac{\tau}{\tau_{0}} \right) \left(\frac{2}{\tau} + \frac{1}{\tau_{0}}\right) \right] 
%\\
%&\left[ \mathbf{v}_{ij} - \frac{\left\|\mathbf{v}_{ij}\right\|^{2} \mathbf{x}_{ij} - \left(\mathbf{x}_{ij}\cdot\mathbf{v}_{ij}\right) \mathbf{v}_{ij} }{\sqrt{\left(\mathbf{x}_{ij}\cdot\mathbf{v}_{ij}\right)^{2} - \left\|\mathbf{v}_{ij}\right\|^{2} \left( \left\|\mathbf{x}_{ij}\right\|^{2} - r_{ij}^{2} \right) }} \right]
&= - \left(\frac{k}{a \tau^{2}}\right) 
\left(\frac{2}{\tau} + \frac{1}{\tau_{0}}\right) 
\exp\left (-\frac{\tau}{\tau_{0}}\right )
\left(\mathbf{v}_{ij} -\frac{a \mathbf{x}_{ij} + b \mathbf{v}_{ij}}{d} \right) 
\end{align}



